block_equiv_checker_soundness.v
@@ -105,179 +105,77 @@ Import Constraints.
 Require Import FORVES2.context.
 Import Context.
 
+Require Import FORVES2.tools_types.
+Import ToolsTypes.
+
 From Coq Require Import Lists.List. Import ListNotations.
 
 Module BlockEquivCheckerSoundness.
 
-Lemma evm_eq_block_chkr'_snd: forall
-    (memory_updater: smemory_updater_ext_type) 
-    (storage_updater: sstorage_updater_ext_type)
-    (mload_solver: mload_solver_ext_type) 
-    (sload_solver: sload_solver_ext_type)
-    (sstack_value_cmp_ext: sstack_val_cmp_ext_2_t)
-    (smemory_cmp_ext: smemory_cmp_ext_t)
-    (sstorage_cmp_ext: sstorage_cmp_ext_t)
-    (sha3_cmp_ext: sha3_cmp_ext_t)
+  Lemma evm_eq_block_chkr'_snd: forall
+    (tools: Tools.tools_t)
     (imp_chkr: imp_checker)
     (opt_pipeline: opt_pipeline)
     (opt_step_rep: nat)
     (opt_pipeline_rep: nat),
-    smemory_updater_ext_snd memory_updater ->
-    sstorage_updater_ext_snd storage_updater ->
-    mload_solver_ext_snd mload_solver ->
-    sload_solver_ext_snd sload_solver ->
-    sstack_val_cmp_fail_for_d_eq_0 sstack_value_cmp_ext ->
-    safe_smemory_cmp_ext_wrt_sstack_value_cmp smemory_cmp_ext ->
-    safe_sstorage_cmp_ext_wrt_sstack_value_cmp sstorage_cmp_ext ->
-    safe_sha3_cmp_ext_wrt_sstack_value_cmp sha3_cmp_ext ->
-    safe_sstack_value_cmp_wrt_others sstack_value_cmp_ext ->
 
-    eq_block_chkr_snd (evm_eq_block_chkr' memory_updater storage_updater mload_solver sload_solver sstack_value_cmp_ext smemory_cmp_ext sstorage_cmp_ext sha3_cmp_ext imp_chkr opt_pipeline opt_step_rep opt_pipeline_rep).
+    eq_block_chkr_snd (evm_eq_block_chkr' tools imp_chkr opt_pipeline opt_step_rep opt_pipeline_rep).
 Proof.
-  intros memory_updater storage_updater mload_solver sload_solver sstack_value_cmp_ext smemory_cmp_ext sstorage_cmp_ext sha3_cmp_ext imp_chkr opt_pipeline opt_step_rep opt_pipeline_rep H_smemory_updater_ext_snd H_sstorage_updater_ext_snd H_mload_solver_ext_snd H_sload_solver_ext_snd H_sstack_val_cmp_fail_for_d_eq_0 H_safe_smemory_cmp_ext_wrt_sstack_value_cmp H_safe_sstorage_cmp_ext_wrt_sstack_value_cmp H_safe_sha3_cmp_ext_wrt_sstack_value_cmp H_safe_sstack_value_cmp_wrt_others.
-
-  (* combining the comparators results in a sound one *)
-  pose proof (safe_all_cmp smemory_cmp_ext sstorage_cmp_ext sha3_cmp_ext sstack_value_cmp_ext H_sstack_val_cmp_fail_for_d_eq_0 H_safe_smemory_cmp_ext_wrt_sstack_value_cmp H_safe_sstorage_cmp_ext_wrt_sstack_value_cmp H_safe_sha3_cmp_ext_wrt_sstack_value_cmp H_safe_sstack_value_cmp_wrt_others) as H_safe_all_cmp.
+  intros tools imp_chkr opt_pipeline opt_step_rep opt_pipeline_rep.
+  destruct tools eqn:H_tools.
+  rewrite <- H_tools.
 
   unfold eq_block_chkr_snd.
+  
   intros p1 p2 cs sst H_evm_eq_block_chkr'.
 
   unfold evm_eq_block_chkr' in H_evm_eq_block_chkr'.
- 
 
   destruct (chk_valid_sstate sst evm_stack_opm) eqn:E_valid_sst_b; try discriminate.
-  
+
   pose proof (chk_valid_sstate_snd sst evm_stack_opm E_valid_sst_b) as H_valid_sst.
   
-  remember (sstack_value_cmp_ext smemory_cmp_ext sstorage_cmp_ext sha3_cmp_ext) as sstack_value_cmp_1.
-  remember (memory_updater sstack_value_cmp_1) as memory_updater'.
+  unfold evm_eq_block_chkr'.
+ 
+  rewrite H_tools in H_evm_eq_block_chkr'.
+  unfold Tools.smemory_updater in H_evm_eq_block_chkr'.
+  unfold Tools.sstorage_updater in H_evm_eq_block_chkr'.
+  unfold Tools.mload_solver in H_evm_eq_block_chkr'.
+  unfold Tools.sload_solver in H_evm_eq_block_chkr'.
 
-  remember (storage_updater sstack_value_cmp_1) as storage_updater'.
-  remember (mload_solver sstack_value_cmp_1) as mload_solver'.
-  remember (sload_solver sstack_value_cmp_1) as sload_solver'.
   remember (mk_ctx imp_chkr cs) as ctx.
 
 
-  destruct (evm_exec_block_s memory_updater' storage_updater' mload_solver' sload_solver' p1 ctx sst evm_stack_opm) as [sst_opt|] eqn:E_sym_exec_p1; try discriminate.
+  destruct (evm_exec_block_s smemory_updater sstorage_updater mload_solver sload_solver p1 ctx sst evm_stack_opm) as [sst_opt|] eqn:E_sym_exec_p1; try discriminate.
 
-  destruct (evm_exec_block_s memory_updater' storage_updater' mload_solver' sload_solver' p2 ctx sst evm_stack_opm) as [sst_p|] eqn:E_sym_exec_p2; try discriminate.
+  destruct (evm_exec_block_s smemory_updater sstorage_updater mload_solver sload_solver p2 ctx sst evm_stack_opm) as [sst_p|] eqn:E_sym_exec_p2; try discriminate.
 
   remember (S (max (get_maxidx_smap (get_smap_sst sst_opt)) (get_maxidx_smap (get_smap_sst sst_p)))) as maxid.
-  remember (sstack_value_cmp_1 maxid) as sstack_value_cmp.
-  remember (apply_opt_n_times_pipeline_k opt_pipeline sstack_value_cmp opt_step_rep opt_pipeline_rep) as opt.
+
+  rewrite <- H_tools in H_evm_eq_block_chkr'.
+
+  destruct (mk_tools_1 tools maxid) eqn:E_tools_1.
+
+  simpl in H_evm_eq_block_chkr'.
+    
+  remember (apply_opt_n_times_pipeline_k opt_pipeline sstack_val_cmp opt_step_rep opt_pipeline_rep) as opt.
 
   destruct (opt ctx sst_opt) as [sst_opt' aux_bool_opt1] eqn:H_sst_opt_apply_op.
   destruct (opt ctx sst_p) as [sst_p' aux_bool_opt2] eqn:H_sst_p_apply_op.
 
-  remember (smemory_cmp_ext sstack_value_cmp) as smemory_cmp.
-  remember (sstorage_cmp_ext sstack_value_cmp) as sstorage_cmp.
+  pose proof (sstate_cmp_snd sstack_val_cmp smemory_cmp sstorage_cmp H_sstack_val_cmp_snd H_smemory_cmp_snd H_sstorage_cmp_snd) as H_sstate_cmp_snd.
 
-  pose proof (safe_ext_all_cmp smemory_cmp_ext sstorage_cmp_ext sha3_cmp_ext sstack_value_cmp_ext H_sstack_val_cmp_fail_for_d_eq_0 H_safe_smemory_cmp_ext_wrt_sstack_value_cmp H_safe_sstorage_cmp_ext_wrt_sstack_value_cmp H_safe_sha3_cmp_ext_wrt_sstack_value_cmp H_safe_sstack_value_cmp_wrt_others) as [H_sstack_value_cmp_ext [H_smemory_cmp_ext [H_sstorage_cmp_ext H_sha3_cmp_ext ]]].
-
-
-  assert (H_sstack_value_cmp_ext_1: forall d, safe_sstack_val_cmp_ext_1_d sstack_value_cmp_1 d).
-  (* proof of assert *)
-  rewrite Heqsstack_value_cmp_1.
-  intros.
-  apply safe_ext_2_implies_safe_ext_1.
-  apply H_sstack_value_cmp_ext.
-  (* end of proof of assert *)
-  
-  assert (H_sstack_value_cmp_ext_1': safe_sstack_val_cmp_ext_1 sstack_value_cmp_1).
-  (* proof of assert *)
-  unfold safe_sstack_val_cmp_ext_1.
-  apply H_sstack_value_cmp_ext_1.
-  (* end of proof of assert *)
-
-  
-  assert (H_memory_updater'_snd: smemory_updater_snd memory_updater').
-  (* proof of assert *)
-  unfold safe_sstack_val_cmp_ext_2 in H_sstack_value_cmp_ext.
-  unfold smemory_updater_ext_snd in H_smemory_updater_ext_snd.
-  pose proof (H_smemory_updater_ext_snd sstack_value_cmp_1 H_sstack_value_cmp_ext_1') as H_smemory_updater_ext_snd'.
-  rewrite <- Heqmemory_updater' in H_smemory_updater_ext_snd'.
-  apply H_smemory_updater_ext_snd'.
-  (* end of proof of assert *)
-
-
-  assert (H_storage_updater'_snd: sstorage_updater_snd storage_updater').
-  (* proof of assert *)
-  unfold safe_sstack_val_cmp_ext_2 in H_sstack_value_cmp_ext.
-  unfold sstorage_updater_ext_snd in H_sstorage_updater_ext_snd.
-  pose proof (H_sstorage_updater_ext_snd sstack_value_cmp_1 H_sstack_value_cmp_ext_1') as H_sstorage_updater_ext_snd'.
-  rewrite <- Heqstorage_updater' in H_sstorage_updater_ext_snd'.
-  apply H_sstorage_updater_ext_snd'.
-  (* end of proof of assert *)
-
-  assert (H_mload_solver'_snd: mload_solver_snd mload_solver').
-  (* proof of assert *)
-  unfold safe_sstack_val_cmp_ext_2 in H_sstack_value_cmp_ext.
-  unfold mload_solver_ext_snd in H_mload_solver_ext_snd.
-  pose proof (H_mload_solver_ext_snd sstack_value_cmp_1 H_sstack_value_cmp_ext_1') as H_mload_solver_ext_snd'.
-  rewrite <- Heqmload_solver' in H_mload_solver_ext_snd'.
-  apply H_mload_solver_ext_snd'.
-  (* end of proof of assert *)
-
-  assert (H_sload_solver'_snd: sload_solver_snd sload_solver').
-  (* proof of assert *)
-  unfold safe_sstack_val_cmp_ext_2 in H_sstack_value_cmp_ext.
-  unfold sload_solver_ext_snd in H_sload_solver_ext_snd.
-  pose proof (H_sload_solver_ext_snd sstack_value_cmp_1 H_sstack_value_cmp_ext_1') as H_sload_solver_ext_snd'.
-  rewrite <- Heqsload_solver' in H_sload_solver_ext_snd'.
-  apply H_sload_solver_ext_snd'.
-  (* end of proof of assert *)
-
-  (* soundness of symbolic execution of p1 *)
-  pose proof (symbolic_exec_snd memory_updater' storage_updater' mload_solver' sload_solver' p1 ctx sst sst_opt evm_stack_opm H_valid_sst H_memory_updater'_snd H_storage_updater'_snd H_mload_solver'_snd H_sload_solver'_snd E_sym_exec_p1) as [H_sym_exc_snd_p1_1 H_sym_exc_snd_p1_2].
-
-  (* soundness of symbolic execution of p2 *)
-  pose proof (symbolic_exec_snd memory_updater' storage_updater' mload_solver' sload_solver' p2 ctx sst sst_p evm_stack_opm H_valid_sst H_memory_updater'_snd H_storage_updater'_snd H_mload_solver'_snd H_sload_solver'_snd E_sym_exec_p2) as [H_sym_exc_snd_p2_1  H_sym_exc_snd_p2_2].
-
-  assert (H_safe_sstack_value_cmp: safe_sstack_val_cmp sstack_value_cmp).
-  (* proof of assert *)
-  unfold  safe_sstack_val_cmp_ext_1 in H_sstack_value_cmp_ext_1'.
-  pose proof (H_sstack_value_cmp_ext_1 maxid) as H_sstack_value_cmp_ext_1'_maxid.
-  unfold safe_sstack_val_cmp_ext_1_d in H_sstack_value_cmp_ext_1'_maxid.
-  pose proof (H_sstack_value_cmp_ext_1'_maxid maxid (PeanoNat.Nat.le_refl maxid)) as H_sstack_value_cmp_ext_1'_maxid.
-  rewrite Heqsstack_value_cmp.
-  apply H_sstack_value_cmp_ext_1'_maxid.
-  (* end of proof of assert *)
-
-  (* opt that is generated by the pipeline is sound *)
-  pose proof (apply_opt_n_times_pipeline_k_snd opt_pipeline sstack_value_cmp opt_step_rep opt_pipeline_rep H_safe_sstack_value_cmp) as H_safe_opt.
-  rewrite <- Heqopt in H_safe_opt.
-
-  assert (H_safe_smemory_cmp: safe_smemory_cmp smemory_cmp).
-  (* proof of assert *)
-  rewrite <- Heqsstack_value_cmp_1 in H_smemory_cmp_ext.
-  unfold safe_smemory_cmp_ext in H_smemory_cmp_ext.
-  pose proof (H_smemory_cmp_ext maxid) as H_smemory_cmp_ext.
-  unfold safe_smemory_cmp_ext_d in H_smemory_cmp_ext.
-  pose proof (H_smemory_cmp_ext maxid (PeanoNat.Nat.le_refl maxid)) as H_smemory_cmp_ext_maxid.
-  rewrite <- Heqsstack_value_cmp in H_smemory_cmp_ext_maxid.
-  rewrite <- Heqsmemory_cmp in H_smemory_cmp_ext_maxid.
-  apply H_smemory_cmp_ext_maxid.
-  (* end of proof of assert *)
-  
-  assert (H_safe_sstorage_cmp: safe_sstorage_cmp sstorage_cmp).
-  (* proof of assert *)
-  rewrite <- Heqsstack_value_cmp_1 in H_sstorage_cmp_ext.
-  unfold safe_sstorage_cmp_ext in H_sstorage_cmp_ext.
-  pose proof (H_sstorage_cmp_ext maxid) as H_sstorage_cmp_ext.
-  unfold safe_sstorage_cmp_ext_d in H_sstorage_cmp_ext.
-  pose proof (H_sstorage_cmp_ext maxid (PeanoNat.Nat.le_refl maxid)) as H_sstorage_cmp_ext_maxid.
-  rewrite <- Heqsstack_value_cmp in H_sstorage_cmp_ext_maxid.
-  rewrite <- Heqsstorage_cmp in H_sstorage_cmp_ext_maxid.
-  apply H_sstorage_cmp_ext_maxid.
-  (* end of proof of assert *)
- 
-  pose proof (sstate_cmp_snd sstack_value_cmp smemory_cmp sstorage_cmp H_safe_sstack_value_cmp H_safe_smemory_cmp H_safe_sstorage_cmp) as H_sstate_cmp_snd.
-  
   unfold sem_eq_blocks.
   intros mem strg exts in_st model H_is_model H_in_st_is_instance_of_sst.
 
   assert (H_ctx_cs: (ctx_cs ctx) = cs). rewrite Heqctx. simpl. reflexivity.
   rewrite <- H_ctx_cs in H_is_model.
+
+  (* soundness of symbolic execution of p1 *)
+  pose proof (symbolic_exec_snd smemory_updater sstorage_updater mload_solver sload_solver p1 ctx sst sst_opt evm_stack_opm H_valid_sst H_smemory_updater_snd H_sstorage_updater_snd H_mload_solver_snd H_sload_solver_snd E_sym_exec_p1) as [H_sym_exc_snd_p1_1 H_sym_exc_snd_p1_2].
+
+  (* soundness of symbolic execution of p2 *)
+  pose proof (symbolic_exec_snd smemory_updater sstorage_updater mload_solver sload_solver p2 ctx sst sst_p evm_stack_opm H_valid_sst H_smemory_updater_snd H_sstorage_updater_snd H_mload_solver_snd H_sload_solver_snd E_sym_exec_p2) as [H_sym_exc_snd_p2_1  H_sym_exc_snd_p2_2].
 
   pose proof (H_sym_exc_snd_p1_2 mem strg exts in_st model H_is_model H_in_st_is_instance_of_sst) as H_sym_exc_snd_p1_2.
   destruct H_sym_exc_snd_p1_2 as [st'_1 [H_sym_exc_snd_p1_2_1 H_sym_exc_snd_p1_2_2]].
@@ -287,6 +185,10 @@ Proof.
 
   exists st'_1. exists st'_2.
   split; try split; try apply H_sym_exc_snd_p1_2_1; try apply H_sym_exc_snd_p2_2_1.
+
+    (* opt that is generated by the pipeline is sound *)
+  pose proof (apply_opt_n_times_pipeline_k_snd opt_pipeline sstack_val_cmp opt_step_rep opt_pipeline_rep H_sstack_val_cmp_snd) as H_safe_opt.
+  rewrite <- Heqopt in H_safe_opt.
 
   unfold optim_snd in H_safe_opt.
 
@@ -359,6 +261,8 @@ Proof.
     reflexivity.
 Qed.
 
+
+
 Lemma evm_eq_block_chkr_lazy_snd:
   forall (memory_updater_tag: available_smemory_updaters) (storage_updater_tag: available_sstorage_updaters) (mload_solver_tag: available_mload_solvers) 
   (sload_solver_tag: available_sload_solvers) (sstack_value_cmp_tag: available_sstack_val_cmp) (memory_cmp_tag: available_memory_cmp)
@@ -369,21 +273,15 @@ Proof.
   intros memory_updater_tag storage_updater_tag mload_solver_tag sload_solver_tag sstack_value_cmp_tag memory_cmp_tag storage_cmp_tag sha3_cmp_tag imp_chkr_tag optimization_steps opt_step_rep opt_pipeline_rep chkr H_chkr.
 
   unfold evm_eq_block_chkr_lazy in H_chkr.
-  destruct (get_smemory_updater memory_updater_tag) as [smemory_updater H_smemory_updater_snd].
-  destruct (get_sstorage_updater storage_updater_tag) as [sstorage_updater H_sstorage_updater_snd].
-  destruct (get_mload_solver mload_solver_tag) as [mload_solver H_mload_solver_snd].
-  destruct (get_sload_solver sload_solver_tag) as [sload_solver H_sload_solver_snd].
-  destruct (get_sstack_val_cmp sstack_value_cmp_tag) as [sstack_value_cmp H_sstack_value_cmp_snd  H_sstack_value_cmp_snd_d0].
-  destruct (get_memory_cmp memory_cmp_tag) as [smemory_cmp H_smemory_cmp_snd].
-  destruct (get_storage_cmp storage_cmp_tag) as [sstorage_cmp H_sstorage_cmp_snd].
-  destruct (get_sha3_cmp sha3_cmp_tag) as [ssha3_cmp H_ssha3_cmp_snd].
+
+  remember (mk_tools sstack_value_cmp_tag memory_cmp_tag storage_cmp_tag sha3_cmp_tag mload_solver_tag sload_solver_tag memory_updater_tag storage_updater_tag) as tools.
 
   unfold eq_block_chkr_snd.
   intros p1 p2 cs sst H_apply_chkr.
   rewrite <- H_chkr in H_apply_chkr.
   remember (get_impl_chkr imp_chkr_tag cs) as imp_chkr.
   
-  pose proof (evm_eq_block_chkr'_snd smemory_updater sstorage_updater mload_solver sload_solver sstack_value_cmp smemory_cmp sstorage_cmp ssha3_cmp imp_chkr (get_pipeline optimization_steps) opt_step_rep opt_pipeline_rep H_smemory_updater_snd H_sstorage_updater_snd H_mload_solver_snd H_sload_solver_snd H_sstack_value_cmp_snd_d0 H_smemory_cmp_snd H_sstorage_cmp_snd H_ssha3_cmp_snd H_sstack_value_cmp_snd) as H_evm_eq_block_chkr'_snd.
+  pose proof (evm_eq_block_chkr'_snd tools imp_chkr (get_pipeline optimization_steps) opt_step_rep opt_pipeline_rep) as H_evm_eq_block_chkr'_snd.
   unfold eq_block_chkr_snd in H_evm_eq_block_chkr'_snd.
   apply H_evm_eq_block_chkr'_snd.
   apply H_apply_chkr.
