tools_types.v
@@ -1,0 +1,96 @@
+
+
+Require Import FORVES2.storage_ops_solvers.
+Import StorageOpsSolvers.
+
+Require Import FORVES2.memory_ops_solvers.
+Import MemoryOpsSolvers.
+
+Require Import FORVES2.symbolic_state_cmp.
+Import SymbolicStateCmp.
+
+
+(* Record to encapsulate all comparators, solvers, updaters, etc. -- no used yet *)
+Module ToolsTypes.
+
+Module Tools.
+Record tools_t : Type := 
+  {
+    (* stack value comparator -- recieves recursion depth and comparators for mem/strg/sha3 *)
+    sstack_val_cmp_ext_2 : sstack_val_cmp_ext_2_t;
+    H_sstack_val_cmp_ext_2_snd: safe_sstack_value_cmp_wrt_others sstack_val_cmp_ext_2;
+    H_sstack_val_cmp_ext_2_d0_snd: sstack_val_cmp_fail_for_d_eq_0 sstack_val_cmp_ext_2;
+
+    (* memory comparator -- recieves sstack_val_cmp_ext_1_t *)
+    smemory_cmp_ext : smemory_cmp_ext_t;
+    H_smemory_cmp_ext_snd: safe_smemory_cmp_ext_wrt_sstack_value_cmp smemory_cmp_ext;
+    (* storage comparator -- recieves sstack_val_cmp_ext_1_t *)
+    sstorage_cmp_ext : sstorage_cmp_ext_t;
+    H_sstorage_cmp_ext_snd: safe_sstorage_cmp_ext_wrt_sstack_value_cmp sstorage_cmp_ext;
+
+    (* sha3 comparator -- recieves sstack_val_cmp_ext_1_t *)
+    sha3_cmp_ext : sha3_cmp_ext_t;
+    H_sha3_cmp_ext_snd: safe_sha3_cmp_ext_wrt_sstack_value_cmp sha3_cmp_ext;
+
+    (* stack value comparator -- recieves recursion depth *)
+    sstack_val_cmp_ext_1 : sstack_val_cmp_ext_1_t;
+    H_sstack_val_cmp_ext_1_snd: safe_sstack_val_cmp_ext_1 sstack_val_cmp_ext_1;
+
+    (* mload solver -- recieves sstack_val_cmp_ext_1_t *)
+    mload_solver_ext : mload_solver_ext_type;
+    H_mload_solver_ext_snd : mload_solver_ext_snd mload_solver_ext;
+
+    (* sload solver -- recieves sstack_val_cmp_ext_1_t *)
+    sload_solver_ext : sload_solver_ext_type;
+    H_sload_solver_ext_snd : sload_solver_ext_snd sload_solver_ext;
+
+    (* memory updater -- recieves sstack_val_cmp_ext_1_t *)
+    smemory_updater_ext : smemory_updater_ext_type;
+    H_smemory_updater_ext_snd : smemory_updater_ext_snd smemory_updater_ext;
+
+    (* storage updater -- recieves sstack_val_cmp_ext_1_t *)
+    sstorage_updater_ext : sstorage_updater_ext_type;
+    H_sstorage_updater_ext_snd : sstorage_updater_ext_snd sstorage_updater_ext;
+
+    (* mload solver *)
+    mload_solver : mload_solver_type;
+    H_mload_solver_snd : mload_solver_snd mload_solver;
+
+    (* sload solver  *)
+    sload_solver : sload_solver_type;
+    H_sload_solver_snd : sload_solver_snd sload_solver;
+
+    (* memory updater *)
+    smemory_updater : smemory_updater_type;
+    H_smemory_updater_snd : smemory_updater_snd smemory_updater;
+
+    (* storage updater *)
+    sstorage_updater : sstorage_updater_type;
+    H_sstorage_updater_snd : sstorage_updater_snd sstorage_updater;
+  }.
+
+
+End Tools.
+     
+Module Tools_1.
+Record tools_1_t : Type := 
+  {
+    tools : Tools.tools_t;
+
+    (* stack value comparator *)
+    sstack_val_cmp : sstack_val_cmp_t;
+    H_sstack_val_cmp_snd: safe_sstack_val_cmp sstack_val_cmp;
+
+    (* memory comparator *)
+    smemory_cmp : smemory_cmp_t;
+    H_smemory_cmp_snd: safe_smemory_cmp smemory_cmp;
+
+    (* storage comparator *)
+    sstorage_cmp : sstorage_cmp_t;
+    H_sstorage_cmp_snd: safe_sstorage_cmp sstorage_cmp;
+  }.
+End Tools_1.
+
+End ToolsTypes.
+
+      
